simplified ast to cfg phase (always return a CFG) and adjusted acyclicity proof

AstToCfg_simple.dfy
@@ -25,112 +25,93 @@ module AstToCfg {
 
   /** 
     Transforms the Ast `c` into a Cfg.
-    `precedingBlock`: The current basic block that is being processed
-    `currentScope`: Basic block id for current block
-    `labelToBlock`: Basic block ids for all labels in scope
     `nextVersion`: basic block id that is not reserved (including all ids larger than this one)
 
     returns:
-      a Cfg if more than one block was completely processed
+      a cfg 
       next free version
-      Exit block still under construction (if there is such a block)
+      exit block of returned cfg 
   */
-  function method AstToCfgAux(
-    c: Cmd, 
-    precedingBlock: (BlockId, BasicBlock), 
-    nextVersion: BlockId) : (Option<Cfg>, BlockId, Option<(BlockId, BasicBlock)>) //Option for exit block needed once break statements are taken into account
+  function method AstToCfgAux(c: Cmd, nextVersion: BlockId) : (Cfg, BlockId, Option<BlockId>) 
+    //Option for exit block needed once break statements are taken into account
     requires NoBreaksScopesLoops(c)
-    requires precedingBlock.0 < nextVersion
-    ensures  var res := AstToCfgAux(c, precedingBlock, nextVersion); 
-             var exitBlockOpt := res.2;
-             var nextVersion' := res.1;
-             && (exitBlockOpt != None)
-             && (if res.0 == None then 
-                    && nextVersion == nextVersion' 
-                    && precedingBlock.0 == exitBlockOpt.value.0 
-                 else 
-                  && res.0.value.blocks.Keys == res.0.value.successors.Keys
-                  && nextVersion < nextVersion' 
-                  && (nextVersion <= exitBlockOpt.value.0 < nextVersion')
-                  && res.0.value.successors.Keys <= CoveringSet(nextVersion, nextVersion', {precedingBlock.0}, {exitBlockOpt.value.0})
-                )
+    ensures  var (cfg, nextVersion', exitOpt):= AstToCfgAux(c, nextVersion); 
+                exitOpt != None  &&
+                var exit := exitOpt.value;
+                && cfg.successors.Keys == cfg.blocks.Keys - {exit}
+                && nextVersion < nextVersion' 
+                && (nextVersion <= exit < nextVersion')
+                && cfg.successors.Keys <= CoveringSet2(nextVersion, nextVersion', {exit})
+                && cfg.entry in cfg.blocks.Keys
+                && exit in cfg.blocks.Keys
   {
     match c
-    case SimpleCmd(simpleC) => (None, nextVersion, Some((precedingBlock.0, precedingBlock.1+[simpleC])))
-    case Seq(thn, els) =>
-      var (optCfg1, nextVersion1, optExit1) := AstToCfgAux(thn, precedingBlock, nextVersion);
+    case SimpleCmd(simpleC) =>
+      (Cfg(nextVersion, map[nextVersion := simpleC], map[]), nextVersion+1, Some(nextVersion))
+    case Seq(c1, c2) =>
+      var (cfg1, nextVersion1, exitOpt1) := AstToCfgAux(c1, nextVersion);
+      if exitOpt1.None? then
+        //c2 will never be reached
+        (cfg1, nextVersion1, exitOpt1)
+      else 
+        var (cfg2, nextVersion2, exitOpt2) := AstToCfgAux(c2, nextVersion1);
 
-      if optExit1.None? then
-        //els will never be reached
-        (optCfg1, nextVersion1, optExit1)
-      else
-        var (optCfg2, nextVersion2, optExit2) := AstToCfgAux(els, optExit1.value, nextVersion1);
+        //merge cfgs
+        var cover1 := CoveringSet2(nextVersion, nextVersion1, {exitOpt1.value});
+        var cover2 := CoveringSet2(nextVersion1, nextVersion2, {exitOpt2.value});
+        var cover3 := CoveringSet2(nextVersion, nextVersion2, {exitOpt2.value});
+        assert cover1 + cover2 <= cover3;
 
-        if optCfg1.None? then
-          //since the exit block for thn becomes the preceding block for els, we can take the result for els
-          assert optCfg2.Some? ==> nextVersion == nextVersion1 && optExit1.value.0 == precedingBlock.0;
-          (optCfg2, nextVersion2, optExit2)
-        else if optCfg2.None? then
-          var cfg1 := optCfg1.value;
-          assert optExit2.value.0 == optExit1.value.0;
-          assert nextVersion1 == nextVersion2;
-          (optCfg1, nextVersion2, optExit2)
-        else
-          //merge cfgs
-          var cfg1 := optCfg1.value;
-          var cfg2 := optCfg2.value;
-
-          var cover1 := CoveringSet(nextVersion, nextVersion1, {precedingBlock.0}, {optExit1.value.0});
-          var cover2 := CoveringSet(nextVersion1, nextVersion2, {optExit1.value.0}, {optExit2.value.0});
-          var cover3 := CoveringSet(nextVersion, nextVersion2, {precedingBlock.0}, {optExit2.value.0});
-          assert cover1 + cover2 <= cover3;
-
-          (Some(Cfg(cfg1.entry, cfg1.blocks + cfg2.blocks, cfg1.successors + cfg2.successors)), nextVersion2, optExit2)
+        var successors := (cfg1.successors + cfg2.successors)[exitOpt1.value := [cfg2.entry]];
+  
+        (Cfg(cfg1.entry, cfg1.blocks + cfg2.blocks, successors), nextVersion2, exitOpt2)
     case If(optCond, thn, els) => 
       /** CFG thn branch */
-      var (thnStartId, thnStartBlock) := if optCond.Some? then (nextVersion, [Assume(optCond.value)]) else (nextVersion, []);
-      var (optCfg1, nextVersion1, optExit1) := AstToCfgAux(thn, (thnStartId, thnStartBlock), nextVersion+1);
+      var (entryId, entryBlock) := (nextVersion, Skip);
+      var (cfgThn, nextVersion1, exitOpt1) := AstToCfgAux(thn, entryId+1);
+
+      var cfgThn' := 
+        if optCond.Some? then
+          Cfg(cfgThn.entry, cfgThn.blocks[cfgThn.entry := SeqSimple(Assume(optCond.value), cfgThn.blocks[cfgThn.entry])], cfgThn.successors)
+        else
+          cfgThn;
 
       /** CFG els branch */
-      var (elsStartId, elsStartBlock) := if optCond.Some? then (nextVersion1, [Assume(UnOp(Not, optCond.value))]) else (nextVersion1, []);
-      var (optCfg2, nextVersion2, optExit2) := AstToCfgAux(els, (elsStartId, elsStartBlock), nextVersion1+1);
+      var (cfgEls, nextVersion2, exitOpt2) := AstToCfgAux(els, nextVersion1);
+
+      var cfgEls' := 
+        if optCond.Some? then
+          Cfg(cfgEls.entry, cfgEls.blocks[cfgEls.entry := SeqSimple(Assume(UnOp(Not, optCond.value)), cfgEls.blocks[cfgEls.entry])], cfgEls.successors)
+        else
+          cfgEls;
 
       /** 
-        * precedingBlock is the entry block 
-        * connect precedingBlock to thnStartId and elsStartId
+        * connect entry block to thnStartId and elsStartId
         * if then/else branch have active exit blocks, then connect those to a fresh basic block, which will became the active basic block
       */
-      var (entryBlockId, entryBlock) := precedingBlock;
 
       /** new successor relation */
       var (blocksThnEls, successorsThnEls) := 
-        if optCfg1.Some? && optCfg2.Some? then
-          (optCfg1.value.blocks + optCfg2.value.blocks, optCfg1.value.successors + optCfg2.value.successors)
-        else if optCfg1.Some? then
-          (optCfg1.value.blocks, optCfg1.value.successors)
-        else if optCfg2.Some? then
-          (optCfg2.value.blocks, optCfg2.value.successors)
-        else
-          (map[], map[]);
+        (cfgThn'.blocks + cfgEls'.blocks, cfgThn'.successors + cfgEls'.successors);
 
-      var blocksBeforeJoin := blocksThnEls[entryBlockId := entryBlock]; 
-      var successorsBeforeJoin := successorsThnEls[entryBlockId := [thnStartId, elsStartId]];
+      var blocksBeforeJoin := blocksThnEls[entryId := entryBlock]; 
+      var successorsBeforeJoin := successorsThnEls[entryId := [cfgThn'.entry, cfgEls'.entry]];
 
-      if optExit1.Some? && optExit2.Some? then
+      if exitOpt1.Some? && exitOpt2.Some? then
         //connect the end of both branches to a new block
-        var (joinId, joinBlock) := (nextVersion2, []);
-        var (thnExitId, thenExitBlock) := optExit1.value;
-        var (elsExitId, elseExitBlock) := optExit2.value;
+        var (joinId, joinBlock) := (nextVersion2, Skip);
+        var thnExit := exitOpt1.value;
+        var elsExit := exitOpt2.value;
 
-        var blocks := blocksBeforeJoin[thnExitId := thenExitBlock][elsExitId := elseExitBlock];
-        var successors := successorsBeforeJoin[thnExitId := [joinId]][elsExitId := [joinId]];
-        var cfg := Cfg(entryBlockId, blocks, successors);
+        var blocks := blocksBeforeJoin[joinId := joinBlock];
+        var successors := successorsBeforeJoin[thnExit := [joinId]][elsExit := [joinId]];
+        var cfg := Cfg(entryId, blocks, successors);
 
-        (Some(cfg), nextVersion2+1, Some((joinId, joinBlock)))
+        (cfg, nextVersion2+1, Some(joinId))
       else 
-        var cfg := Cfg(entryBlockId, blocksBeforeJoin, successorsBeforeJoin);
-        var optExitResult := if optExit1.Some? then optExit1 else optExit2;
-        (Some(cfg), nextVersion2, optExitResult)
+        var cfg := Cfg(entryId, blocksBeforeJoin, successorsBeforeJoin);
+        var exitOptResult := if exitOpt1.Some? then exitOpt1 else exitOpt2;
+        (cfg, nextVersion2, exitOptResult)
   }
 
   function CoveringSet(oldVersion: nat, newVersion: nat, including: set<nat>, excluding: set<nat>) : set<nat>
@@ -138,99 +119,93 @@ module AstToCfg {
     ((set x : nat | oldVersion <= x < newVersion) + including) - excluding
   }
 
+  function CoveringSet2(oldVersion: nat, newVersion: nat, exclude: set<nat>) : set<nat>
+  {
+    (set x : nat | oldVersion <= x < newVersion) - exclude
+  }
+
   lemma AstToCfgAcyclic(
     c: Cmd, 
-    precedingBlock: (BlockId, BasicBlock), 
     nextVersion: BlockId)
     requires NoBreaksScopesLoops(c)
-    requires precedingBlock.0 < nextVersion
     ensures  
-      var res := AstToCfgAux(c, precedingBlock, nextVersion); 
-      var nextVersion' := res.1;
-      var (exitBlockId, exitBlock) := res.2.value;
+      var (cfg, nextVersion', exitOpt):= AstToCfgAux(c, nextVersion); 
 
-      if res.0.Some? then  
-        var cfg := res.0.value;
-        var s := cfg.successors;
-        
-        && cfg.entry == precedingBlock.0
-        && (forall n :: n in s.Keys ==>   
-            (forall i :: 0 <= i < |s[n]| ==> (s[n][i] == exitBlockId || s[n][i] in s.Keys))) 
-        && cfg.entry in s.Keys 
-        && IsAcyclic(cfg.successors, cfg.entry, CoveringSet(nextVersion, nextVersion', {precedingBlock.0}, {exitBlockId}))
-
-      else  
-        precedingBlock.0 == exitBlockId 
-        //TODO: && precedingBlock.1 <= exitBlock
+      var exit := exitOpt.value;
+      var s := cfg.successors;
+      
+      && (forall n :: n in s.Keys ==>   
+          (forall i :: 0 <= i < |s[n]| ==> (s[n][i] == exit || s[n][i] in s.Keys))) 
+      && cfg.entry in cfg.blocks.Keys 
+      && IsAcyclic(cfg.successors, cfg.entry, CoveringSet2(nextVersion, nextVersion', {exit}))
   {
     match c {
-      case SimpleCmd(_) => 
-      case Seq(thn, els) =>
-        var (optCfg1, nextVersion1, optExit1) := AstToCfgAux(thn, precedingBlock, nextVersion);
+      case SimpleCmd(sc) =>  assume false;
+      case Seq(c1, c2) =>
+        assume false;
+        var (cfg1, nextVersion1, exitOpt1) := AstToCfgAux(c1, nextVersion);
+        var exit1 := exitOpt1.value;
+        assert IsAcyclic(cfg1.successors, cfg1.entry, CoveringSet2(nextVersion, nextVersion1, {exit1}));
 
-        if optExit1.None? {
-          //els will never be reached
-          //this case cannot occur in the simplified setting
-          assert false;
-        } else {
-          var (optCfg2, nextVersion2, optExit2) := AstToCfgAux(els, optExit1.value, nextVersion1);
-          AstToCfgAcyclic(els, optExit1.value, nextVersion2);
+        var (cfg2, nextVersion2, exitOpt2) := AstToCfgAux(c2, nextVersion1);
+        AstToCfgAcyclic(c2, nextVersion2);
 
-          var (exitBlockId2, exitBlock2) := optExit2.value;
+        var exit2 := exitOpt2.value;
 
-          if optCfg1.None? {
-            //since the exit block for thn becomes the preceding block for els, we can take the result for els
-            //(optCfg2, nextVersion2, optExit2)
-            if optCfg2.Some? {
-              var cfg2 := optCfg2.value;
-              
-              IsAcyclicLargerCover(
-                cfg2.successors, 
-                cfg2.entry, 
-                CoveringSet(nextVersion1, nextVersion2, {optExit1.value.0}, {exitBlockId2}), 
-                CoveringSet(nextVersion, nextVersion2, {optExit1.value.0}, {exitBlockId2})
-              );
-            }
-          } else if optCfg2.None? {
-            //(optCfg1, nextVersion2, optExit2)
-          } else {
-            //merge cfgs
-            var cfg1 := optCfg1.value;
-            var cfg2 := optCfg2.value;
+        //merge cfgs
 
-            var cover1 := CoveringSet(nextVersion, nextVersion1, {precedingBlock.0}, {cfg2.entry});
-            var cover2 := CoveringSet(nextVersion1, nextVersion2, {cfg2.entry}, {exitBlockId2});
-            var cover3 := CoveringSet(nextVersion, nextVersion2, {precedingBlock.0}, {exitBlockId2});
+        var cover1 := CoveringSet2(nextVersion, nextVersion1, {exit1});
+        var cover2 := CoveringSet2(nextVersion1, nextVersion2, {exit2});
+        var cover3 := CoveringSet2(nextVersion, nextVersion2, {exit2});
 
-            assert cover1 !! cover2;
-            assert cfg1.successors.Keys !! cfg2.successors.Keys;
 
-            IsAcyclicMerge(
-              cfg1.successors, cfg2.successors, cfg1.entry, cfg2.entry, 
-              cover1,
-              cover2
-              );
+        var successors := (cfg1.successors + cfg2.successors)[exitOpt1.value := [cfg2.entry]];
+        assert successors == (cfg1.successors[exitOpt1.value := [cfg2.entry]] + cfg2.successors);
 
-            IsAcyclicLargerCover(cfg1.successors + cfg2.successors, cfg1.entry, cover1 + cover2, cover3);
-          }
-        }
+        assert cover1 !! cover2;
+        assert cfg1.successors.Keys !! cfg2.successors.Keys;
+
+        IsAcyclicUpdate2(cfg1.successors, cfg1.entry, exit1, [cfg2.entry], cover1);
+
+        assert IsAcyclic(cfg1.successors[exit1 := [cfg2.entry]], cfg1.entry, cover1+{exit1});
+
+        IsAcyclicMerge(
+          cfg1.successors[exit1 := [cfg2.entry]], cfg2.successors, cfg1.entry, cfg2.entry, 
+          cover1+{exit1},
+          cover2
+          );
+
+        IsAcyclicLargerCover(successors, cfg1.entry, (cover1 + {exit1}) + cover2, cover3);
       case If(optCond, thn, els) => 
-        var (thnStartId, thnStartBlock) := if optCond.Some? then (nextVersion, [Assume(optCond.value)]) else (nextVersion, []);
-        var (optCfg1, nextVersion1, optExit1) := AstToCfgAux(thn, (thnStartId, thnStartBlock), nextVersion+1);
+        /** CFG thn branch */
+        var (entryId, entryBlock) := (nextVersion, Skip);
+        var (cfgThn, nextVersion1, exitOpt1) := AstToCfgAux(thn, entryId+1);
 
-        var (elsStartId, elsStartBlock) := if optCond.Some? then (nextVersion1, [Assume(UnOp(Not, optCond.value))]) else (nextVersion1, []);
-        var (optCfg2, nextVersion2, optExit2) := AstToCfgAux(els, (elsStartId, elsStartBlock), nextVersion1+1);
+        var cfgThn' := 
+          if optCond.Some? then
+            Cfg(cfgThn.entry, cfgThn.blocks[cfgThn.entry := SeqSimple(Assume(optCond.value), cfgThn.blocks[cfgThn.entry])], cfgThn.successors)
+          else
+            cfgThn;
 
-        var exit1 := optExit1.value;
-        var exit2 := optExit2.value;
+        /** CFG els branch */
+        var (cfgEls, nextVersion2, exitOpt2) := AstToCfgAux(els, nextVersion1);
 
-        var (entry1, s1) := if optCfg1.Some? then (optCfg1.value.entry, optCfg1.value.successors) else (exit1.0, map[]);
-        var (entry2, s2) := if optCfg2.Some? then (optCfg2.value.entry, optCfg2.value.successors) else (exit2.0, map[]);
+        var cfgEls' := 
+          if optCond.Some? then
+            Cfg(cfgEls.entry, cfgEls.blocks[cfgEls.entry := SeqSimple(Assume(UnOp(Not, optCond.value)), cfgEls.blocks[cfgEls.entry])], cfgEls.successors)
+          else
+            cfgEls;
 
-        var cover1 := CoveringSet(nextVersion+1, nextVersion1, {nextVersion}, {exit1.0});
+        var (entry1, s1) := (cfgThn.entry, cfgThn.successors);
+        var thnExit := exitOpt1.value;
+
+        var cover1 := CoveringSet2(nextVersion+1, nextVersion1, {thnExit});
         assert IsAcyclic(s1, entry1, cover1);
 
-        var cover2 := CoveringSet(nextVersion1+1, nextVersion2, {nextVersion1}, {exit2.0});
+        var (entry2, s2) := (cfgEls.entry, cfgEls.successors);
+        var elsExit := exitOpt2.value;
+
+        var cover2 := CoveringSet2(nextVersion1, nextVersion2, {elsExit});
         assert IsAcyclic(s2, entry2, cover2);
 
         IsAcyclicExtend2(s1, s2, entry1, cover1);
@@ -241,73 +216,39 @@ module AstToCfg {
         IsAcyclicLargerCover(s1 + s2, entry2, cover2, cover1+cover2);
         assert IsAcyclic(s1 + s2, entry2, cover1+cover2);
 
-        var (entryBlockId, entryBlock) := precedingBlock;
+        var successorsBeforeJoin := (s1 + s2)[entryId := [cfgThn'.entry, cfgEls'.entry]];
 
-        var successorsBeforeJoin := (s1 + s2)[entryBlockId := [thnStartId, elsStartId]];
-
-        assert IsAcyclic(successorsBeforeJoin, entryBlockId, cover1+cover2+{entryBlockId}) by {
+        assert IsAcyclic(successorsBeforeJoin, entryId, cover1+cover2+{entryId}) by {
           calc {
-            IsAcyclic(successorsBeforeJoin, entryBlockId, cover1+cover2+{entryBlockId});
-            IsAcyclicSeq(successorsBeforeJoin, [thnStartId, elsStartId], cover1+cover2);
-            IsAcyclic(successorsBeforeJoin, thnStartId, cover1+cover2) &&
-            IsAcyclicSeq(successorsBeforeJoin, [elsStartId], cover1+cover2);
-            IsAcyclic(successorsBeforeJoin, thnStartId, cover1+cover2) &&
-            IsAcyclic(successorsBeforeJoin, elsStartId, cover1+cover2);
-            { IsAcyclicUpdate(s1+s2, entry1, entryBlockId, [thnStartId, elsStartId], cover1+cover2);
-              IsAcyclicUpdate(s1+s2, entry2, entryBlockId, [thnStartId, elsStartId], cover1+cover2);
+            IsAcyclic(successorsBeforeJoin, entryId, cover1+cover2+{entryId});
+            IsAcyclicSeq(successorsBeforeJoin, [cfgThn'.entry, cfgEls'.entry], cover1+cover2);
+            IsAcyclic(successorsBeforeJoin, cfgThn'.entry, cover1+cover2) &&
+            IsAcyclicSeq(successorsBeforeJoin, [cfgEls'.entry], cover1+cover2);
+            IsAcyclic(successorsBeforeJoin, cfgThn'.entry, cover1+cover2) &&
+            IsAcyclic(successorsBeforeJoin, cfgEls'.entry, cover1+cover2);
+            { IsAcyclicUpdate(s1+s2, entry1, entryId, [cfgThn'.entry, cfgEls'.entry], cover1+cover2);
+              IsAcyclicUpdate(s1+s2, entry2, entryId, [cfgThn'.entry, cfgEls'.entry], cover1+cover2);
             }
-            IsAcyclic(s1+s2, thnStartId, cover1+cover2) &&
-            IsAcyclic(s1+s2, elsStartId, cover1+cover2);
+            IsAcyclic(s1+s2, cfgThn'.entry, cover1+cover2) &&
+            IsAcyclic(s1+s2, cfgEls'.entry, cover1+cover2);
           }
         }
 
-        var (thnExitId, thenExitBlock) := optExit1.value;
-        var (elsExitId, elseExitBlock) := optExit2.value;
+        IsAcyclicUpdate2(successorsBeforeJoin, entryId, thnExit, [nextVersion2], cover1+cover2+{entryId});
+        IsAcyclicUpdate2(successorsBeforeJoin[thnExit := [nextVersion2]], entryId, elsExit, [nextVersion2], cover1+cover2+{entryId}+{thnExit});
 
-        IsAcyclicUpdate2(successorsBeforeJoin, entryBlockId, thnExitId, [nextVersion2], cover1+cover2+{entryBlockId});
-        IsAcyclicUpdate2(successorsBeforeJoin[thnExitId := [nextVersion2]], entryBlockId, elsExitId, [nextVersion2], cover1+cover2+{entryBlockId}+{thnExitId});
+        var successorsBeforeJoinImpl := (s1+s2)[entryId := [cfgThn'.entry, cfgEls'.entry]];
 
+        var successors := successorsBeforeJoinImpl[thnExit := [nextVersion2]][elsExit := [nextVersion2]];
+        var cover3 := cover1+cover2+{entryId}+{thnExit}+{elsExit};
 
-        var successorsBeforeJoinImpl := 
-          if optCfg1.Some? && optCfg2.Some? then
-            (s1+s2)[entryBlockId := [thnStartId, elsStartId]]
-          else if optCfg1.Some? then
-            s1[entryBlockId := [thnStartId, elsStartId]]
-          else if optCfg2.Some? then
-            s2[entryBlockId := [thnStartId, elsStartId]]
-          else 
-            (map[])[entryBlockId := [thnStartId, elsStartId]];
-
-        var successors := successorsBeforeJoinImpl[thnExitId := [nextVersion2]][elsExitId := [nextVersion2]];
-        var cover3 := cover1+cover2+{entryBlockId}+{thnExitId}+{elsExitId};
-
-        assert IsAcyclic(successors, entryBlockId, cover3) by {
-          assert successors == successorsBeforeJoin[thnExitId := [nextVersion2]][elsExitId := [nextVersion2]];
+        assert IsAcyclic(successors, entryId, cover3) by {
+          assert successors == successorsBeforeJoin[thnExit := [nextVersion2]][elsExit := [nextVersion2]];
         }
         
-        assert IsAcyclic(successors, entryBlockId, CoveringSet(nextVersion, nextVersion2+1, {precedingBlock.0}, {nextVersion2})) by {
-          assert cover3 == CoveringSet(nextVersion, nextVersion2+1, {precedingBlock.0}, {nextVersion2});
+        assert IsAcyclic(successors, entryId, CoveringSet2(nextVersion, nextVersion2+1, {nextVersion2})) by {
+          assert cover3 == CoveringSet2(nextVersion, nextVersion2+1, {nextVersion2});
         }
     }
   }           
-
-  /*
-  lemma AstToCfgSimpleCorrect<A>(
-    a: absval_interp<A>,
-    c: Cmd, 
-    precedingBlock: (BlockId, BasicBlock), 
-    nextVersion: BlockId,
-    post: Predicate<Cmd>,
-    s: state<A>) 
-    requires NoBreaksScopesLoops(c)
-    ensures  var res := AstToCfgAux(c, precedingBlock, nextVersion); 
-             if res.0.Some? then  
-              var cfg := res.0.value;
-              WpShallow(a, c, WpPostShallow(post, post, map[]))(s) == WpCfg(a, cfg, cfg.entry, post)(s)
-             else 
-              //res.1.Some?
-              true
-  */
-
-
 }
